cont

Experiments/IO_Tree.thy
@@ -2,147 +2,361 @@ theory IO_Tree
 imports FSM
 begin
 
-datatype 'a IO_Tree = IO_Tree 'a "'a IO_Tree list" 
-datatype 'a IO_Tree_Set = IO_Tree_Set "'a \<Rightarrow> 'a IO_Tree option"
+subsection \<open>Utils\<close>
 
-fun node_value :: "'a IO_Tree \<Rightarrow> 'a" where
-  "node_value (IO_Tree a ts) = a"
+fun update_assoc_list_with_default :: "'a \<Rightarrow> ('b \<Rightarrow> 'b) \<Rightarrow> 'b \<Rightarrow> ('a \<times> 'b) list \<Rightarrow> ('a \<times> 'b) list" where
+  "update_assoc_list_with_default k f d [] = [(k,f d)]" |
+  "update_assoc_list_with_default k f d ((x,y)#xys) = (if k = x
+    then ((x,f y)#xys)
+    else (x,y) # (update_assoc_list_with_default k f d xys))"
 
-fun from_list :: "'a \<Rightarrow> 'a list \<Rightarrow> 'a IO_Tree" where
-  "from_list a [] = (IO_Tree a [])" |
-  "from_list a (x#xs) = (IO_Tree a [from_list x xs])"
-
-fun insert :: "'a \<Rightarrow> 'a list \<Rightarrow> 'a IO_Tree \<Rightarrow> 'a IO_Tree" where
-  "insert a [] t = t" |
-  "insert a (x#xs) (IO_Tree y ts) = (if a = y 
-    then case find_remove (\<lambda> t . node_value t = x) ts of
-      Some (t,ts') \<Rightarrow> (IO_Tree y ((insert x xs t)#ts')) |
-      None         \<Rightarrow> (IO_Tree y ((from_list x xs)#ts))
-    else (IO_Tree y ts))"
-
-value "from_list 0 [1::nat,2,3,4,5]"
-value "insert 0 [1,30,80] (from_list 0 [1::nat,2,3,4,5])"
-value "insert 0 [1,30,90] (insert 0 [1,30,80] (from_list 0 [1::nat,2,3,4,5]))"
-
-
-
-fun paths :: "'a IO_Tree \<Rightarrow> 'a list list" where
-  "paths (IO_Tree a []) = [[a]]" |
-  "paths (IO_Tree a (t#ts)) = map ((#) a) (concat (map paths (t#ts)))" 
-
-value "paths (insert 0 [1,30,90] (insert 0 [1,30,80] (from_list 0 [1::nat,2,3,4,5])))"
-
-
-lemma path_from_list :
-  "paths (from_list t p) = [(t#p)]"
-  by (induction p arbitrary: t; auto)
-
-
-
-(* TODO: write induction scheme based on tree height *)
-
-fun max_elem_value_nat_fun :: "('a \<Rightarrow> nat) \<Rightarrow> 'a \<Rightarrow> 'a list \<Rightarrow> nat" where
-  "max_elem_value_nat_fun f x xs = max (f x) (foldr (\<lambda> x' prev_max . max (f x') prev_max) xs 0)"
-
-lemma max_elem_value_nat_fun_ex :
-  "\<exists> x' . x' \<in> set (x#xs) \<and> max_elem_value_nat_fun f x xs = f x'"
-proof (induction xs)
+lemma update_assoc_list_with_default_key_found :
+  assumes "distinct (map fst xys)"
+  and     "i < length xys"
+  and     "fst (xys ! i) = k"
+shows "update_assoc_list_with_default k f d xys =
+        ((take i xys) @ [(k, f (snd (xys ! i)))] @ (drop (Suc i) xys))" 
+using assms proof (induction xys arbitrary: i)
   case Nil
   then show ?case by auto
 next
-  case (Cons a xs)
-  then show ?case 
+  case (Cons a xys)
+  
+  show ?case
+  proof (cases i)
+    case 0
+    then have "fst a = k" using Cons.prems(3) by auto
+    then have "update_assoc_list_with_default k f d (a#xys) = (k, f (snd a)) # xys"
+      unfolding 0 by (metis prod.collapse update_assoc_list_with_default.simps(2)) 
+    then show ?thesis unfolding 0 by auto
+  next
+    case (Suc j)
+    then have "fst a \<noteq> k"
+      using Cons.prems by auto 
+
+    have "distinct (map fst xys)"
+    and  "j < length xys"
+    and  "fst (xys ! j) = k"
+      using Cons.prems unfolding Suc by auto
+
+    then have "update_assoc_list_with_default k f d xys = take j xys @ [(k, f (snd (xys ! j)))] @ drop (Suc j) xys"
+      using Cons.IH[of j] by auto
+
+    then show ?thesis unfolding Suc using \<open>fst a \<noteq> k\<close>
+      by (metis append_Cons drop_Suc_Cons nth_Cons_Suc prod.collapse take_Suc_Cons update_assoc_list_with_default.simps(2)) 
+  qed 
+qed 
+
+lemma update_assoc_list_with_default_key_not_found :
+  assumes "distinct (map fst xys)"
+  and     "k \<notin> set (map fst xys)"
+shows "update_assoc_list_with_default k f d xys = xys @ [(k,f d)]"  
+  using assms by (induction xys; auto)
+
+
+lemma update_assoc_list_with_default_key_distinct :
+  assumes "distinct (map fst xys)"
+  shows "distinct (map fst (update_assoc_list_with_default k f d xys))"
+proof (cases "k \<in> set (map fst xys)")
+  case True
+  then obtain i where "i < length xys" and "fst (xys ! i) = k"
+    by (metis in_set_conv_nth length_map nth_map) 
+  then have *: "(map fst (take i xys @ [(k, f (snd (xys ! i)))] @ drop (Suc i) xys)) = (map fst xys)"
+  proof -
+    have "xys ! i # drop (Suc i) xys = drop i xys"
+      using Cons_nth_drop_Suc \<open>i < length xys\<close> by blast
+    then show ?thesis
+      by (metis (no_types) \<open>fst (xys ! i) = k\<close> append_Cons append_self_conv2 append_take_drop_id fst_conv list.simps(9) map_append)
+  qed
+  show ?thesis
+    unfolding update_assoc_list_with_default_key_found[OF assms \<open>i < length xys\<close> \<open>fst (xys ! i) = k\<close>] * 
+    using assms by assumption
+next
+  case False
+  have *: "(map fst (xys @ [(k, f d)])) = (map fst xys)@[k]" by auto
+  show ?thesis
+    using assms False
+    unfolding update_assoc_list_with_default_key_not_found[OF assms False] * by auto
 qed
 
-end (*
-
-fun height :: "'a IO_Tree \<Rightarrow> nat" where
-  "height (IO_Tree a []) = 0" |
-  "height (IO_Tree a (t#ts)) = 
 
 
-lemma paths_non_nil :
-  "paths t \<noteq> []"
+
+
+
+subsection \<open>IO Tries\<close>
+
+
+datatype 'a io_trie = IO_Trie "('a \<times> 'a io_trie) list"
+
+fun io_trie_invar :: "'a io_trie \<Rightarrow> bool" where
+  "io_trie_invar (IO_Trie ts) = (distinct (map fst ts) \<and> (\<forall> t \<in> set (map snd ts) . io_trie_invar t))"
+
+
+
+definition empty :: "'a io_trie" where
+  "empty = IO_Trie []"
+
+lemma empty_invar : "io_trie_invar empty" unfolding empty_def by auto
+
+
+
+fun height :: "'a io_trie \<Rightarrow> nat" where
+  "height (IO_Trie []) = 0" |
+  "height (IO_Trie (xt#xts)) = Suc (foldr (\<lambda> t m . max (height t) m) (map snd (xt#xts)) 0)"
+
+lemma height_0 : 
+  assumes "height t = 0" 
+  shows "t = empty" 
+proof (rule ccontr)
+  assume "t \<noteq> empty"
+  then obtain xt xts where "t = IO_Trie (xt#xts)"
+    by (metis IO_Tree.empty_def height.cases)
+  have "height t > 0" 
+    unfolding \<open>t = IO_Trie (xt#xts)\<close> height.simps
+    by simp
+  then show "False"
+    using assms by simp
+qed
+
+
+lemma max_by_foldr :
+  assumes "x \<in> set xs"
+  shows "f x < Suc (foldr (\<lambda> x' m . max (f x') m) xs 0)"
+  using assms by (induction xs; auto)
+
+lemma height_inc :
+  assumes "t \<in> set (map snd ts)"
+  shows "height t < height (IO_Trie ts)"
 proof -
-  obtain a ts where "t = IO_Tree a ts"
-    using IO_Tree.exhaust by auto 
-  then show ?thesis proof (cases ts; auto)
+  obtain xt xts where "ts = xt#xts"
+    using assms
+    by (metis list.set_cases list_map_source_elem) 
+  
+  have "height t < Suc (foldr (\<lambda> t m . max (height t) m) (map snd (xt#xts)) 0)"
+    using assms unfolding \<open>ts = xt#xts\<close> using max_by_foldr[of t "(map snd (xt#xts))" height] 
+    by blast
 
-lemma path_insert_set : 
-  "set (paths (insert x xs (IO_Tree x ts))) = Set.insert (x#xs) (set (paths (IO_Tree x ts)) - {p' . \<exists> p'' .  (x#xs) = p'@p''})"
-proof (induction xs arbitrary: x ts)
+  then show ?thesis unfolding \<open>ts = xt#xts\<close> by auto
+qed
+
+(*
+lemma io_tree_induct :
+  assumes "P empty"
+  and     "\<And> ts . (\<And> t . t \<in> set (map snd ts) \<Longrightarrow> P t) \<Longrightarrow> P (IO_Trie ts)"
+shows "P t"
+*)
+
+
+
+
+
+fun insert :: "'a list \<Rightarrow> 'a io_trie \<Rightarrow> 'a io_trie" where
+  "insert [] t = t" |
+  "insert (x#xs) (IO_Trie ts) = (IO_Trie (update_assoc_list_with_default x (\<lambda> t . insert xs t) (IO_Trie []) ts))"
+
+
+lemma insert_invar : "io_trie_invar t \<Longrightarrow> io_trie_invar (insert xs t)" 
+proof (induction xs arbitrary: t)
   case Nil
-
-  have "(insert x [] (IO_Tree x ts)) = (IO_Tree x ts)" by auto
-  show ?case proof (cases ts)
-    case Nil
-    then have "paths (IO_Tree x ts) = [[x]]" by auto
-    show ?thesis unfolding \<open>(insert x [] (IO_Tree x ts)) = (IO_Tree x ts)\<close> \<open>paths (IO_Tree x ts) = [[x]]\<close> by auto
-  next
-    case (Cons t ts')
-    have "map paths (t # ts') \<noteq> []" by auto
-
-    have "\<And> t . paths t \<noteq> []" 
-    moreover have "\<And> p . p \<in> set (map paths (t # ts')) \<Longrightarrow> p \<noteq> []" 
-    proof -
-      fix p assume "p \<in> set (map paths (t # ts'))"
-      obtain a' ts'' where "t = IO_Tree a' ts''" 
-
-
-end (*
-    then have "\<And> p . p \<in> set (map ((#) x) (concat (map paths (t # ts')))) \<Longrightarrow> length p > 1" 
-    proof - 
-      fix p assume "p \<in> set (map ((#) x) (concat (map paths (t # ts'))))"
-      then obtain p' where "p' \<in> 
-    then have "[x] \<notin> set (paths (IO_Tree x ts))"  unfolding Cons paths.simps 
-    then show ?thesis sorry
-  qed
-
-  have "{p' . \<exists> p'' .  (x#[]) = p'@p''} = {[],[x]}" 
-
-  then show ?case proof (cases 
+  then show ?case by auto
 next
-  case (Cons a xs)
+  case (Cons x xs)
+
+  obtain ts where "t = IO_Trie ts"
+    using io_trie_invar.cases by auto
+
+  then have "distinct (map fst ts)"
+       and  "\<And> t . t \<in> set (map snd ts) \<Longrightarrow> io_trie_invar t"
+    using Cons.prems by auto
+    
+  
+  show ?case proof (cases "x \<in> set (map fst ts)")
+    case True
+    then obtain i where "i < length ts" and "fst (ts ! i) = x"
+      by (metis in_set_conv_nth length_map nth_map) 
+    have "insert (x#xs) (IO_Trie ts) = (IO_Trie (take i ts @ [(x, insert xs (snd (ts ! i)))] @ drop (Suc i) ts))"
+      unfolding insert.simps
+      unfolding update_assoc_list_with_default_key_found[OF \<open>distinct (map fst ts)\<close> \<open>i < length ts\<close> \<open>fst (ts ! i) = x\<close>, of "(\<lambda> t . insert xs t)" "(IO_Trie [])"] 
+      by simp
+    
+    have "\<And> t . t \<in> set (map snd (take i ts @ [(x, insert xs (snd (ts ! i)))] @ drop (Suc i) ts)) \<Longrightarrow> io_trie_invar t"
+    proof - 
+      fix t assume "t \<in> set (map snd (take i ts @ [(x, insert xs (snd (ts ! i)))] @ drop (Suc i) ts))"
+      then consider (a) "t \<in> set (map snd (take i ts @ drop (Suc i) ts))" |
+                    (b) "t = insert xs (snd (ts ! i))" 
+        by auto
+      then show "io_trie_invar t" proof cases
+        case a
+        then have "t \<in> set (map snd ts)"
+          by (metis drop_map in_set_dropD in_set_takeD list_concat_non_elem map_append take_map) 
+        then show ?thesis using \<open>\<And> t . t \<in> set (map snd ts) \<Longrightarrow> io_trie_invar t\<close> by blast
+      next
+        case b
+        have "(snd (ts ! i)) \<in> set (map snd ts)"
+          using \<open>i < length ts\<close> by auto
+        then have "io_trie_invar (snd (ts ! i))" using \<open>\<And> t . t \<in> set (map snd ts) \<Longrightarrow> io_trie_invar t\<close> by blast 
+        then show ?thesis using Cons.IH unfolding b by blast
+      qed 
+    qed
+    moreover have "distinct (map fst (take i ts @ [(x, insert xs (snd (ts ! i)))] @ drop (Suc i) ts))"
+      using update_assoc_list_with_default_key_distinct[OF \<open>distinct (map fst ts)\<close>]
+      by (metis \<open>distinct (map fst ts)\<close> \<open>fst (ts ! i) = x\<close> \<open>i < length ts\<close> update_assoc_list_with_default_key_found)
+    
+    ultimately show ?thesis 
+      unfolding \<open>t = IO_Trie ts\<close> \<open>insert (x#xs) (IO_Trie ts) = (IO_Trie (take i ts @ [(x, insert xs (snd (ts ! i)))] @ drop (Suc i) ts))\<close>
+      by auto
+  next
+    case False
+
+    have "io_trie_invar (IO_Tree.insert xs (IO_Trie []))"
+      by (induction xs; auto)
+
+    then show ?thesis
+      using Cons.prems update_assoc_list_with_default_key_distinct[OF \<open>distinct (map fst ts)\<close>, of x "(IO_Tree.insert xs)" "(IO_Trie [])"]
+      unfolding \<open>t = IO_Trie ts\<close> insert.simps
+      unfolding update_assoc_list_with_default_key_not_found[OF \<open>distinct (map fst ts)\<close> False] 
+      by auto
+  qed
+qed 
+
+
+
+
+fun paths :: "'a io_trie \<Rightarrow> 'a list list" where
+  "paths (IO_Trie []) = [[]]" |
+  "paths (IO_Trie (t#ts)) = concat (map (\<lambda> (x,t) . map ((#) x) (paths t)) (t#ts))"
+
+
+
+value "insert [1,2,3,4] (empty :: nat io_trie)"
+value "insert [1,2,5,6] (insert [1,2,3,4] (empty :: nat io_trie))"
+value "insert [1,2,5,7] (insert [1,2,5,6] (insert [1,2,3,4] (empty :: nat io_trie)))"
+value "paths (insert [1,2,5,7] (insert [1,2,5,6] (insert [1,2,3,4] (empty :: nat io_trie))))"
+
+
+
+lemma paths_empty :
+  assumes "[] \<in> set (paths t)"
+  shows "t = empty"
+proof (rule ccontr)
+  assume "t \<noteq> empty"
+  then obtain xt xts where "t = IO_Trie (xt#xts)"
+    by (metis IO_Tree.empty_def height.cases)
+  then have "[] \<in> set (concat (map (\<lambda> (x,t) . map ((#) x) (paths t)) (xt#xts)))"
+    using assms by auto
+  then show "False" by auto
+qed
+
+lemma paths_nonempty :
+  assumes "[] \<notin> set (paths t)"
+  shows "set (paths t) \<noteq> {}"
+using assms proof (induction t rule: io_trie_invar.induct)
+  case (1 ts)
+  have "ts \<noteq> []" using "1.prems" by auto
+  then obtain x t xts where "ts = ((x,t)#xts)"
+    using linear_order_from_list_position'.cases
+    by (metis old.prod.exhaust) 
+  
+  then have "t \<in> set (map snd ts)" by auto
+    
+  show ?case 
+  proof (cases "[] \<in> set (paths t)")
+    case True
+    then show ?thesis  
+      unfolding \<open>ts = ((x,t)#xts)\<close> paths.simps by auto
+  next
+    case False
+    show ?thesis 
+      using "1.IH"[OF \<open>t \<in> set (map snd ts)\<close> False]  
+      unfolding \<open>ts = ((x,t)#xts)\<close> paths.simps by auto
+  qed
+qed
+
+
+lemma paths_maximal: "io_trie_invar t \<Longrightarrow> xs' \<in> set (paths t) \<Longrightarrow> \<not> (\<exists> xs'' . xs'' \<noteq> [] \<and> xs'@xs'' \<in> set (paths t))"
+proof (induction xs' arbitrary: t)
+  case Nil
+  then have "t = empty"
+    using paths_empty by blast
+  then have "paths t = [[]]"
+    by (simp add: empty_def)
+  then show ?case by auto
+next
+  case (Cons x xs')
+
+  then have "t \<noteq> empty" unfolding empty_def by auto
+  then obtain xt xts where "t = IO_Trie (xt#xts)"
+    by (metis IO_Tree.empty_def height.cases)
+
+  obtain t' where "(x,t') \<in> set (xt#xts)"
+            and   "xs' \<in> set (paths t')"
+    using Cons.prems(2) 
+    unfolding \<open>t = IO_Trie (xt#xts)\<close> paths.simps 
+    by force
+
+  have "io_trie_invar t'"
+    using Cons.prems(1) \<open>(x,t') \<in> set (xt#xts)\<close> unfolding \<open>t = IO_Trie (xt#xts)\<close> by auto
+
+  show ?case 
+  proof 
+    assume "\<exists>xs''. xs'' \<noteq> [] \<and> (x # xs') @ xs'' \<in> set (paths t)"
+    then obtain xs'' where "xs'' \<noteq> []" and "(x # (xs' @ xs'')) \<in> set (paths (IO_Trie (xt # xts)))"
+      unfolding \<open>t = IO_Trie (xt#xts)\<close> by force
+
+
+    obtain t'' where "(x,t'') \<in> set (xt#xts)"
+               and   "(xs' @ xs'') \<in> set (paths t'')"
+      using \<open>(x # (xs' @ xs'')) \<in> set (paths (IO_Trie (xt # xts)))\<close>
+      unfolding \<open>t = IO_Trie (xt#xts)\<close> paths.simps 
+      by force
+
+    have "distinct (map fst (xt#xts))"
+      using Cons.prems(1) unfolding \<open>t = IO_Trie (xt#xts)\<close> by simp
+    then have "t'' = t'"
+      using \<open>(x,t') \<in> set (xt#xts)\<close> \<open>(x,t'') \<in> set (xt#xts)\<close>
+      by (meson eq_key_imp_eq_value)  
+    then have "xs'@xs'' \<in> set (paths t')"
+      using \<open>(xs' @ xs'') \<in> set (paths t'')\<close> by auto
+    then show "False"
+      using \<open>xs'' \<noteq> []\<close> Cons.IH[OF \<open>io_trie_invar t'\<close> \<open>xs' \<in> set (paths t')\<close>] by blast
+  qed
+qed
+            
+
+
+
+
+
+lemma "io_trie_invar t \<Longrightarrow> set (paths (insert xs t)) = {xs' . xs' \<in> Set.insert xs (set (paths t)) \<and> \<not> (\<exists> xs'' . xs'' \<noteq> [] \<and> xs'@xs'' \<in> Set.insert xs (set (paths t)))}"
+proof (induction xs arbitrary: t)
+  case Nil
+  show ?case proof (cases "[] \<in> set (paths t)")
+    case True
+    have "paths t = [[]]"
+      using paths_empty[OF True] unfolding empty_def by auto
+    show ?thesis using paths_maximal[OF Nil] unfolding insert.simps \<open>paths t = [[]]\<close> by auto
+  next
+    case False
+    then have "\<exists> xs''. xs'' \<noteq> [] \<and> [] @ xs'' \<in> Set.insert [] (set (paths t))"  
+      using paths_nonempty[OF False]
+      by (metis all_not_in_conv append.left_neutral insert_iff) 
+    then have *: "{xs' \<in> Set.insert [] (set (paths t)). \<nexists>xs''. xs'' \<noteq> [] \<and> xs' @ xs'' \<in> Set.insert [] (set (paths t))}
+                = {xs' \<in> (set (paths t)). \<nexists>xs''. xs'' \<noteq> [] \<and> xs' @ xs'' \<in> (set (paths t))}"
+      by blast
+    
+    show ?thesis 
+      using paths_maximal[OF Nil] unfolding insert.simps * by blast
+  qed
+next
+  case (Cons x xs)
   then show ?case sorry
 qed
 
 
-
-end (* 
-
-
-
-lemma path_insert_set : 
-  "set (paths (insert x xs (IO_Tree x ts))) 
-    = (if (\<exists> p' . ((x#xs)@p') \<in> set (paths (insert x xs (IO_Tree x ts))) \<and> p' \<noteq> []) 
-        then set (paths (IO_Tree x ts))
-        else Set.insert p (set (paths (IO_Tree x ts)) - {p' . \<exists> p'' .  p = p'@p''}))"
-
-
-lemma path_insert :
-  "\<exists> p' . ((x#xs)@p') \<in> set (paths (insert x xs (IO_Tree x ts)))" 
-proof (cases "find_remove (\<lambda> t . node_value t = x) ts")
-  case None
-  then show ?thesis then have 
-next
-  case (Some a)
-  then show ?thesis sorry
-qed
-
-
-
 end (*
 
-lemma path_insert_set : "set (paths (insert x xs (IO_Tree x ts))) = (if (\<exists> p' . ((x#xs)@p') \<in> set (paths (insert x xs (IO_Tree x ts))) \<and> p' \<noteq> []) 
-                then set (paths (IO_Tree x ts))
-                else insert p (set (paths (IO_Tree x ts)) - {p' . prefix p' p}))"
-
-
-lemma path_insert_fold:
-  sth like: folding all lists in list of lists into a tree_set contains (exactly) all maximal lists of the original list of lists as paths
-
-
-
+fold-insert over list/set of sequences \<rightarrow> show that all maximal sequences are contained
 
 
 end 
